ref_impl/src/verifier/bosqueTerms.fst
@@ -1,0 +1,193 @@
+module BosqueTerms
+
+open Sequence
+open BosqueTypes
+
+(* Dynamic: depends on the 
+   entities created by user *) 
+type bosqueTerm = 
+| BNone : bosqueTerm
+| BBool : bool -> bosqueTerm
+| BInt : int -> bosqueTerm
+// No support for Float
+// No support for Regex
+| BTypedString : value:string -> content_type:bosqueType -> bosqueTerm
+| BGUID : string -> int -> bosqueTerm
+| BTuple : n:nat -> sequence bosqueTerm n -> bosqueTerm
+| BRecord : n:nat -> sequence bosqueTerm n -> bosqueTerm
+| BError : bosqueTerm
+
+(* Definition of getType *)
+val getTypeSeq : n:nat -> (x: sequence bosqueTerm n) -> Tot (sequence bosqueType n) (decreases x)
+val getType : x:bosqueTerm -> Tot bosqueType (decreases x)
+let rec getType x = match x with
+| BNone -> BNoneType
+| BBool _ -> BBoolType
+| BInt _ -> BIntType
+| BTypedString _ content_type -> BTypedStringType content_type
+| BGUID _ _ -> BGUIDType
+| BTuple n y -> BTupleType false n (getTypeSeq n y)
+// FIX: The following is incomplete
+| BRecord _ _ -> BRecordType false 0 SNil
+| BError -> BErrorType
+and
+getTypeSeq n x = match x with
+| SNil -> SNil
+| SCons y m ys -> SCons (getType y) m (getTypeSeq m ys)
+
+(* --------------------------------------------------------------- *)
+(* Casting / Type checkers *)
+val isNone : bosqueTerm -> Tot bool
+let isNone x = match x with 
+| BNone -> true
+| _ -> false
+
+val isSome : bosqueTerm -> Tot bool
+let isSome x = not (isNone x)
+
+val isBool : bosqueTerm -> Tot bool
+let isBool x = match x with 
+| BBool _ -> true
+| _ -> false 
+
+val isInt : bosqueTerm -> Tot bool
+let isInt x = match x with 
+| BInt _ -> true
+| _ -> false 
+
+val isTypedString : bosqueType -> bosqueTerm -> Tot bool
+let isTypedString ty x = match x with 
+| BTypedString _ ty' -> eqType ty ty'
+| _ -> false 
+
+val isGUID : bosqueTerm -> Tot bool
+let isGUID x = match x with 
+| BGUID _ _ -> true
+| _ -> false 
+
+val isTuple : b:bool -> n:nat -> (sequence bosqueType n) -> x:bosqueTerm -> Tot bool
+let isTuple b n seqTypes x = match x with
+| BTuple m seqTerms -> (n = m) && eqType (BTupleType b n seqTypes) (getType x)
+| _ -> false
+
+val isTuple2 : b:bool -> n:nat -> (sequence bosqueType n) -> x:bosqueTerm -> Tot bool
+let isTuple2 b n seqTypes x = match x with
+| BTuple m seqTerms -> eqType (BTupleType b n seqTypes) (getType x)
+| _ -> false
+
+val isTuple3 : b:bool -> n:nat -> (sequence bosqueType n) -> x:bosqueTerm -> Tot bool
+let isTuple3 b n seqTypes x = eqType (BTupleType b n seqTypes) (getType x)
+
+val isRecord : b:bool -> n:nat -> (sequence bosqueType n) -> x:bosqueTerm -> Tot bool
+let isRecord b n seqTypes x = eqType (getType x) (BRecordType b n seqTypes)
+
+val isError : bosqueTerm -> Tot bool
+let isError x = match x with 
+| BError -> true
+| _ -> false 
+(* --------------------------------------------------------------- *)
+
+(* ------------------------------------------------------------------------ *)
+(* Extractors *)
+
+(* This is mainly used inside conditionals (in the fstar programming language) 
+   and assertions (in the z3 smt solver) *)
+val extractBool : x:bosqueTerm{isBool x} -> Tot bool
+let extractBool x = match x with
+| BBool y -> y 
+
+// Hmmm
+val extractBool2 : x:bosqueTerm{eqType BBoolType (getType x)} -> Tot bool
+let extractBool2 x = match x with
+| BBool y -> y 
+
+// Hmmm2
+val extractBool3 : x:bosqueTerm{subtypeOf BBoolType (getType x)} -> Tot bool
+let extractBool3 x = match x with
+| BBool y -> y 
+(* ------------------------------------------------------------------------ *)
+
+(* Definition of equality relation on Bosque terms *)
+val eqTerm_aux : n:nat 
+  -> (x:sequence bosqueTerm n) 
+  -> sequence bosqueTerm n 
+  -> Tot (z:bosqueTerm{isBool z \/ isError z}) (decreases x)
+val eqTerm : x:bosqueTerm 
+  -> bosqueTerm 
+  -> Tot (z:bosqueTerm{isBool z \/ isError z})  (decreases x)
+let rec eqTerm x y = match x, y with
+| BNone, BNone -> BBool true
+| BBool x1, BBool y1 -> BBool (x1 = y1)
+| BInt x1, BInt y1 -> BBool (x1 = y1)
+| BTypedString s1 ty1, BTypedString s2 ty2 -> BBool (s1 = s2 && eqType ty1 ty2)
+| BGUID s1 n1, BGUID s2 n2 -> BBool (s1 = s2 && n1 = n2)
+| BTuple n1 seq1, BTuple n2 seq2 -> if (n1 <> n2) then BError
+                                   else eqTerm_aux n1 seq1 seq2
+// FIX: Include case for BRecord
+// | BError, BError -> BBool true
+| _, _ -> BError
+and 
+eqTerm_aux n x y = match x with
+| SNil -> (match y with
+         | SNil -> BBool true
+         | _ -> BError
+         )
+| SCons x1 m xs1 -> (match y with
+                   | SNil -> BError
+                   | SCons y1 m' ys1 -> (match (eqTerm x1 y1) with
+                                       | BBool b1 -> (match (eqTerm_aux m xs1 ys1) with
+                                                    | BBool b2 -> BBool ((m = m') && b1 && b2)
+                                                    | _ -> BError
+                                                    )
+                                       | _ -> BError 
+                                       )
+                   )
+
+(* Definition of greater than or equal relation on Bosque terms *)
+val greaterOrEq : x:bosqueTerm{isInt x} -> y:bosqueTerm{isInt x} -> Tot (x:bosqueTerm{isBool x \/ isError x})
+let greaterOrEq x y = match x, y with
+| BInt x1, BInt y1 -> BBool (x1 >= y1)
+// TODO: Include case for Strings
+| _, _ -> BError
+
+(* Tuple Type projector *)
+val nthTupleType : index:int -> dimension:nat -> x:bosqueTerm -> Tot (bosqueType)
+let rec nthTupleType index dimension y = match y with
+| BTuple 0 SNil -> if (index < 0 || dimension <> 0) then BErrorType else BNoneType
+| BTuple dimension'' (SCons x dimension' xs) -> 
+  if (index < 0 || dimension <> dimension'') then BErrorType else
+  if (index >= dimension) then BNoneType else
+  if index = 0 then getType x
+  else nthTupleType (index-1) dimension' (BTuple dimension' xs)
+| _ -> BErrorType
+
+(* Tuple projector *)
+val nthTuple : index:int -> dimension:nat -> x:bosqueTerm -> Tot (y:bosqueTerm)
+let rec nthTuple index dimension y = match y with
+| BTuple 0 SNil -> if (index < 0 || dimension <> 0) then BError else BNone
+| BTuple dimension'' (SCons x' dimension' xs') -> 
+  if (index < 0 || dimension <> dimension'') then BError else
+  if (index >= dimension) then BNone else
+  if index = 0 then x'
+  else nthTuple (index-1) dimension' (BTuple dimension' xs')
+| _ -> BError
+
+// TODO: Implement the Record Projector
+// (* Record projector *)
+// val nthRecord : index:int -> dimension:nat -> bosqueTerm -> Tot bosqueTerm
+// let rec nthRecord index dimension y = match y with
+// | BTuple 0 SNil -> if (index < 0 || dimension <> 0) then BError else BNone
+// | BTuple dimension'' (SCons x #dimension' xs) -> 
+//   if (index < 0 || dimension <> dimension'') then BError else
+//   if (index >= dimension) then BNone else
+//   if index = 0 then x
+//   else nthTuple (index-1) dimension' (BTuple dimension' xs)
+// | _ -> BError
+
+(* ------------------------------------------------------------------------------------------- *)
+(* Type instantiation *)
+type typeUnionIntBool = x:bosqueType{subtypeOf (BUnionType BIntType BBoolType) x}
+type termUnionIntBool = x:bosqueTerm{subtypeOf (BUnionType BIntType BBoolType) (getType x)}
+(* Definition of IntType *)
+type termInt = x:bosqueTerm{isInt x} 
+(* ------------------------------------------------------------------------------------------- *)
