ref_impl/src/verifier/bosqueTypes.fst
@@ -1,0 +1,132 @@
+module BosqueTypes
+
+open Sequence
+module Util=Util
+
+// Convention with UnionTerm: 
+// 1) its elements should be unique
+// 2) There is a unique way to represent any union (normal form)
+// the latter was needed for eqType
+type bosqueType =
+| BAnyType
+| BSomeType
+| BTruthyType
+| BNoneType
+| BUnionType : bosqueType -> bosqueType -> bosqueType
+| BParseableType
+| BBoolType
+| BIntType
+| BFloatType // Bad news, FStar doesn't provide support for this type
+| BRegexType // Bad news, FStar doesn't provide support for this type
+| BTypedStringType : bosqueType -> bosqueType
+| BGUIDType
+// The bool indicates if the Tuple is open or not
+| BTupleType : bool -> n:nat -> sequence bosqueType n -> bosqueType
+// FIX: The following is wrong
+// The bool indicates if the Record is open or not
+| BRecordType : bool -> n:nat -> sequence bosqueType n -> bosqueType
+// FIX: The following is incomplete
+| BFunctionType
+// FIX: The following is incomplete
+| BObjectType
+// FIX: The following is incomplete
+| BEnumType 
+// FIX: The following is incomplete
+| BCustomKeyType
+// FIX: The following is incomplete
+| BKeyedType
+| BErrorType
+
+(* Definition of equality relation on Bosque types *)
+val eqTypeSeq : n:nat -> (x:sequence bosqueType n) -> sequence bosqueType n -> Tot bool (decreases x)
+val eqType : x:bosqueType -> bosqueType -> Tot bool (decreases x)
+let rec eqType x y = match x, y with
+| BAnyType, BAnyType -> true
+| BSomeType, BSomeType -> true
+| BTruthyType, BTruthyType -> true
+| BNoneType, BNoneType -> true
+// The following might be incomplete, but if Unions are normalized then it is complete
+| BUnionType x1 x2 , BUnionType y1 y2 -> eqType x1 y1 && eqType x2 y2
+| BParseableType, BParseableType -> true 
+| BBoolType, BBoolType -> true
+| BIntType, BIntType -> true
+| BFloatType, BFloatType -> true
+| BRegexType, BRegexType -> true
+| BTypedStringType t1, BTypedStringType t2 -> (eqType t1 t2)
+| BGUIDType, BGUIDType -> true 
+| BTupleType b1 n1 seq1, BTupleType b2 n2 seq2 -> (b1 = b2) && (n1 = n2) && eqTypeSeq n1 seq1 seq2
+// FIX: The following is wrong
+| BRecordType _ _ _, BRecordType _ _ _ -> true
+// FIX: The following is incomplete
+| BFunctionType, BFunctionType -> true
+// FIX: The following is incomplete
+| BObjectType, BObjectType -> true
+// FIX: The following is incomplete
+| BEnumType, BEnumType -> true
+// FIX: The following is incomplete
+| BCustomKeyType, BCustomKeyType -> true
+// FIX: The following is incomplete
+| BKeyedType, BKeyedType -> true
+| BErrorType, BErrorType -> true
+| _, _ -> false
+and
+eqTypeSeq n x y = match x with
+| SNil -> (match y with 
+         | SNil -> true
+         | _ -> false
+         )
+| SCons x1 m xs1 -> (match y with 
+                   | SNil -> false
+                   | SCons y1 m' ys1 -> (m = m') && eqType x1 y1 && eqTypeSeq m xs1 ys1
+                   )
+
+(* Definition to encode the subtype relation on Bosque types 
+   i.e. forall x y . subtypeOf x y <===> x :> y *)
+val subtypeOfSeq : n:nat -> (x:sequence bosqueType n) -> sequence bosqueType n -> Tot bool (decreases x)
+val subtypeOf : x:bosqueType -> bosqueType -> Tot bool (decreases x)
+let rec subtypeOf x y = match x, y with
+| BAnyType, _ -> true
+| BSomeType, BAnyType -> false
+| BSomeType, BTruthyType -> false
+| BSomeType, BNoneType -> false
+| BSomeType, _ -> true
+| BTruthyType, BNoneType -> true
+| BNoneType, BNoneType -> true
+| BUnionType x1 y1, BUnionType x2 y2 -> (subtypeOf x1 x2 || subtypeOf y1 x2)
+  && (subtypeOf x1 y2 || subtypeOf y1 y2)
+| BUnionType x1 y1, z -> subtypeOf x1 z || subtypeOf y1 z 
+// | BParseabletype, ? -> ?
+| BBoolType, BBoolType -> true
+| BIntType, BIntType -> true
+// | BFloatType, ? -> ?
+// | BRegexType, ? -> ?
+| BTypedStringType t1, BTypedStringType t2 -> subtypeOf t1 t2
+| BTupleType b1 0 SNil, BTupleType b2 0 SNil -> b1 = b2
+| BTupleType b1 0 SNil, BTupleType _ _ _ -> b1
+| BTupleType b1 n1 seq1, BTupleType b2 n2 seq2 -> 
+  if b1 then 
+    if (n1 > n2) then false
+    else b1 && (n1 <= n2) && subtypeOfSeq n1 seq1 (take n2 n1 seq2)
+  else 
+    if b2 then false 
+    else 
+      if (n1 = n2) then (not b1) && (not b2) && (n1 = n2) && subtypeOfSeq n1 seq1 seq2
+      else false 
+// | BRecordType, ? -> ?
+// | BFunctionType, ? -> ?
+// | BObjectType, ? -> ?
+// | BEnumType, ? -> ?
+// | BCustomType, ? -> ?
+// | BKeyedType, ? -> ?
+| BErrorType, BErrorType -> true
+| _, _ -> false
+and 
+subtypeOfSeq n x y = match x with
+| SNil -> (match y with
+         | SNil -> true
+         | _ -> false
+         )
+| SCons x1 m xs1 -> (match y with 
+                   | SNil -> false
+                   | SCons y1 m' ys1 -> (m = m') && eqType x1 y1 && eqTypeSeq m xs1 ys1  
+                   )
